Update FreeRTOS_tasks_noasserts_proofs_clz.v

timing/examples/FreeRTOS_tasks_noasserts_proofs_clz.v
@@ -170,6 +170,35 @@ Definition offset_mem_pxCurrentTCB_noverlap_clz (gp : N) mem : Prop :=
             (k + mem Ⓓ[48 + pxCurrentTCB gp mem]) 4
             (gp ⊖ 920 ⊕ (31 ⊖ clz (mem Ⓓ[ gp ⊖ 1920 ]) 32) * 20) 4.
 
+Definition clz_noverlap_sframe (gp base_sp : N) mem : Prop :=
+    ~ overlap 32 
+        (base_sp ⊖ 16) 16
+        (gp ⊖ 920 ⊕ (31 ⊖ clz (mem Ⓓ[ gp ⊖ 1920 ]) 32) * 20) 4.
+
+Definition mem4_pxCurrentTCB_noverlap_stackframe gp base_sp mem :=
+        ~ overlap 32
+        (base_sp ⊖ 16) 16
+            (4 + mem Ⓓ[gp ⊖ 920 ⊕ (31 ⊖ clz (mem Ⓓ[ gp ⊖ 1920 ]) 32) * 20]) 4.
+
+Definition mem4_pxCurrentTCB_noverlap_static gp mem :=
+    forall x len_x,
+        static_buffer_lengths_in_bytes x = Some len_x ->
+        ~ overlap 32
+            (gp ⊖ x) 4
+            (4 + mem Ⓓ[gp ⊖ 920 ⊕ (31 ⊖ clz (mem Ⓓ[ gp ⊖ 1920 ]) 32) * 20]) 4.
+
+Definition mem4_mem4_noverlap_stackframe gp base_sp mem :=
+    ~ overlap 32
+        (base_sp ⊖ 16) 16
+        (4 + mem Ⓓ[ 4 + mem Ⓓ[ gp ⊖ 920 ⊕ (31 ⊖ clz (mem Ⓓ[ gp ⊖ 1920 ]) 32) * 20 ] ]) 4.
+
+Definition mem4_mem4_noverlap_static gp mem :=
+    forall x len_x,
+        static_buffer_lengths_in_bytes x = Some len_x ->
+        ~ overlap 32
+            (gp ⊖ x) 4
+            (4 + mem Ⓓ[ 4 + mem Ⓓ[ gp ⊖ 920 ⊕ (31 ⊖ clz (mem Ⓓ[ gp ⊖ 1920 ]) 32) * 20 ] ]) 4.
+
 Definition common_noverlaps gp base_sp mem : Prop :=
     gp_sp_noverlap gp base_sp /\
     smem_well_formed gp /\
@@ -179,13 +208,16 @@ Definition common_noverlaps gp base_sp mem : Prop :=
     clz_noverlap_smem gp mem /\
     mem_pxCurrentTCB_noverlap_stackframe gp base_sp mem /\
     mem_pxCurrentTCB_noverlap_static gp mem /\
-    offset_mem_pxCurrentTCB_noverlap_clz gp mem.
+    offset_mem_pxCurrentTCB_noverlap_clz gp mem /\
+    clz_noverlap_sframe gp base_sp mem /\
+    mem4_pxCurrentTCB_noverlap_stackframe gp base_sp mem /\
+    mem4_pxCurrentTCB_noverlap_static gp mem.
 
 (* TODO : Rewrite postconditions, the if conditions are garbage from earlier versions *)
 Definition timing_postcondition (t : trace) (gp : N) (mem : addr -> N) : Prop :=
     if (uxSchedulerSuspended gp mem) =? 0 then
         cycle_count_of_trace t = 25 + 3 * time_branch + 17 * time_mem
-        + (if (mem Ⓓ[(gp ⊖ 920) ⊕ ((31 ⊖ (clz (uxTopReadyPriority gp mem) 32)) * 20)])
+        + (if (mem Ⓓ[ 4 + mem Ⓓ[ gp ⊖ 920 ⊕ (31 ⊖ clz (uxTopReadyPriority gp mem) 32) * 20 ] ])
             =? ((gp ⊖ 916) ⊕ (31 ⊖ clz (uxTopReadyPriority gp mem) 32) * 20)
             then 22 + clz (mem Ⓓ[ 4294965376 + gp ]) 32 + 5 * time_mem else
             19 + time_branch + clz (mem Ⓓ[ 4294965376 + gp ]) 32 + 3 * time_mem
@@ -193,7 +225,7 @@ Definition timing_postcondition (t : trace) (gp : N) (mem : addr -> N) : Prop :=
     else
         cycle_count_of_trace t = 5 + time_branch + 2 * time_mem.
 
-Definition vTaskSwitchContext_timing_invs (_ : store) (p : addr) (base_sp : N) (t:trace) :=
+Definition vTaskSwitchContext_timing_invs (_ : store) (p : addr) (base_sp gp : N) (base_mem : addr -> N) (t:trace) :=
 match t with (Addr a, s) :: t' => match a with
     (* vApplicationStackOverflowHook *)
     (* NOTE : This function intentionally goes into an infinite loop when a
@@ -203,51 +235,76 @@ match t with (Addr a, s) :: t' => match a with
     | 0x8000e804 => Some True
     (* vTaskSwitchContext *)
     | 0x80001380 => Some (
-        exists mem gp, s V_MEM32 = Ⓜmem /\ s R_GP = Ⓓgp /\ s R_SP = Ⓓbase_sp 
-            /\ s R_A4 = Ⓓ(uxSchedulerSuspended gp mem) /\
+        exists mem, s V_MEM32 = Ⓜmem /\ s R_GP = Ⓓgp /\ s R_SP = Ⓓbase_sp 
+            /\ s R_A4 = Ⓓ(uxSchedulerSuspended gp base_mem) /\
             common_noverlaps gp base_sp mem /\
+            mem4_mem4_noverlap_stackframe gp base_sp mem /\
+            mem4_mem4_noverlap_static gp mem /\
+            uxTopReadyPriority gp mem = uxTopReadyPriority gp base_mem /\
+            mem Ⓓ[ 4 + mem Ⓓ[ gp ⊖ 920 + (31 ⊖ clz (mem Ⓓ[ gp ⊖ 1920 ]) 32) * 20 ] ] =
+            base_mem Ⓓ[ 4 + base_mem Ⓓ[ gp ⊖ 920 + (31 ⊖ clz (base_mem Ⓓ[ gp ⊖ 1920 ]) 32) * 20 ] ]  /\
         cycle_count_of_trace t' = time_mem)
-    | 0x800013b4 => Some (exists mem gp, s V_MEM32 = Ⓜmem /\ 
+    | 0x800013b4 => Some (exists mem, s V_MEM32 = Ⓜmem /\ 
         s R_GP = Ⓓgp /\ s R_SP = Ⓓ(base_sp ⊖ 16) /\
         s R_A5 = Ⓓ(mem Ⓓ[48 + pxCurrentTCB gp mem]) /\
         s R_A2 = Ⓓ(mem Ⓓ[mem Ⓓ[48 + pxCurrentTCB gp mem]]) /\
         s R_A4 = Ⓓ((0xa5a5a << 12) + 1445) /\
         common_noverlaps gp base_sp mem /\
-        (uxSchedulerSuspended gp mem =? 0) = true /\
+        mem4_mem4_noverlap_stackframe gp base_sp mem /\
+        mem4_mem4_noverlap_static gp mem /\
+        uxTopReadyPriority gp mem = uxTopReadyPriority gp base_mem /\
+        mem Ⓓ[ 4 + mem Ⓓ[ gp ⊖ 920 + (31 ⊖ clz (mem Ⓓ[ gp ⊖ 1920 ]) 32) * 20 ] ] =
+        base_mem Ⓓ[ 4 + base_mem Ⓓ[ gp ⊖ 920 + (31 ⊖ clz (base_mem Ⓓ[ gp ⊖ 1920 ]) 32) * 20 ] ]  /\
+        (uxSchedulerSuspended gp base_mem =? 0) = true /\
         cycle_count_of_trace t' = 6 + 7 * time_mem + time_branch)
-    | 0x800013bc => Some (exists mem gp, s V_MEM32 = Ⓜmem /\ 
+    | 0x800013bc => Some (exists mem, s V_MEM32 = Ⓜmem /\ 
         s R_GP = Ⓓgp /\ s R_SP = Ⓓ(base_sp ⊖ 16) /\
         s R_A2 = Ⓓ(mem Ⓓ[mem Ⓓ[48 + pxCurrentTCB gp mem]]) /\
         s R_A3 = Ⓓ(mem Ⓓ[4 + mem Ⓓ[48 + pxCurrentTCB gp mem]]) /\
         s R_A5 = Ⓓ(mem Ⓓ[48 + pxCurrentTCB gp mem]) /\
         common_noverlaps gp base_sp mem /\
-        (uxSchedulerSuspended gp mem =? 0) = true /\
+        mem4_mem4_noverlap_stackframe gp base_sp mem /\
+        mem4_mem4_noverlap_static gp mem /\
+        uxTopReadyPriority gp mem = uxTopReadyPriority gp base_mem /\
+        mem Ⓓ[ 4 + mem Ⓓ[ gp ⊖ 920 + (31 ⊖ clz (mem Ⓓ[ gp ⊖ 1920 ]) 32) * 20 ] ] =
+        base_mem Ⓓ[ 4 + base_mem Ⓓ[ gp ⊖ 920 + (31 ⊖ clz (base_mem Ⓓ[ gp ⊖ 1920 ]) 32) * 20 ] ]  /\
+        (uxSchedulerSuspended gp base_mem =? 0) = true /\
         (mem Ⓓ[ mem Ⓓ[ 48 + pxCurrentTCB gp mem ] ] =? 0xa5a5a5a5) = true /\
         cycle_count_of_trace t' = 9 + 8 * time_mem + time_branch)
-    | 0x800013c4 => Some (exists mem gp, s V_MEM32 = Ⓜmem /\ 
+    | 0x800013c4 => Some (exists mem, s V_MEM32 = Ⓜmem /\ 
         s R_GP = Ⓓgp /\ s R_SP = Ⓓ(base_sp ⊖ 16) /\
         s R_A3 = Ⓓ(mem Ⓓ[4 + mem Ⓓ[48 + pxCurrentTCB gp mem]]) /\
         s R_A4 = Ⓓ(mem Ⓓ[8 + mem Ⓓ[48 + pxCurrentTCB gp mem]]) /\
         s R_A5 = Ⓓ(mem Ⓓ[48 + pxCurrentTCB gp mem]) /\
         common_noverlaps gp base_sp mem /\
+        mem4_mem4_noverlap_stackframe gp base_sp mem /\
+        mem4_mem4_noverlap_static gp mem /\
+        uxTopReadyPriority gp mem = uxTopReadyPriority gp base_mem /\
+        mem Ⓓ[ 4 + mem Ⓓ[ gp ⊖ 920 + (31 ⊖ clz (mem Ⓓ[ gp ⊖ 1920 ]) 32) * 20 ] ] =
+        base_mem Ⓓ[ 4 + base_mem Ⓓ[ gp ⊖ 920 + (31 ⊖ clz (base_mem Ⓓ[ gp ⊖ 1920 ]) 32) * 20 ] ]  /\
         (mem Ⓓ[ mem Ⓓ[ 48 + pxCurrentTCB gp mem ] ] =? 0xa5a5a5a5) = true /\
         (mem Ⓓ[4 + mem Ⓓ[48 + pxCurrentTCB gp mem]] =? mem Ⓓ[mem Ⓓ[48 + pxCurrentTCB gp mem]]) = true /\
-        (uxSchedulerSuspended gp mem =? 0) = true /\
+        (uxSchedulerSuspended gp base_mem =? 0) = true /\
         cycle_count_of_trace t' = 12 + 9 * time_mem + time_branch
     )
-    | 0x800013cc => Some (exists mem gp, s V_MEM32 = Ⓜmem /\ 
+    | 0x800013cc => Some (exists mem, s V_MEM32 = Ⓜmem /\ 
         s R_GP = Ⓓgp /\ s R_SP = Ⓓ(base_sp ⊖ 16) /\
         s R_A3 = Ⓓ(mem Ⓓ[4 + mem Ⓓ[48 + pxCurrentTCB gp mem]]) /\
         s R_A4 = Ⓓ(mem Ⓓ[8 + mem Ⓓ[48 + pxCurrentTCB gp mem]]) /\
         s R_A5 = Ⓓ(mem Ⓓ[12 + mem Ⓓ[48 + pxCurrentTCB gp mem]]) /\
         common_noverlaps gp base_sp mem /\
+        mem4_mem4_noverlap_stackframe gp base_sp mem /\
+        mem4_mem4_noverlap_static gp mem /\
+        uxTopReadyPriority gp mem = uxTopReadyPriority gp base_mem /\
+        mem Ⓓ[ 4 + mem Ⓓ[ gp ⊖ 920 + (31 ⊖ clz (mem Ⓓ[ gp ⊖ 1920 ]) 32) * 20 ] ] =
+        base_mem Ⓓ[ 4 + base_mem Ⓓ[ gp ⊖ 920 + (31 ⊖ clz (base_mem Ⓓ[ gp ⊖ 1920 ]) 32) * 20 ] ]  /\
         (mem Ⓓ[ mem Ⓓ[ 48 + pxCurrentTCB gp mem ] ] =? 0xa5a5a5a5) = true /\
         (mem Ⓓ[4 + mem Ⓓ[48 + pxCurrentTCB gp mem]] =? mem Ⓓ[mem Ⓓ[48 + pxCurrentTCB gp mem]]) = true /\
         (mem Ⓓ[8 + mem Ⓓ[48 + pxCurrentTCB gp mem]] =? mem Ⓓ[4 + mem Ⓓ[48 + pxCurrentTCB gp mem]]) = true /\
-        (uxSchedulerSuspended gp mem =? 0) = true /\
+        (uxSchedulerSuspended gp base_mem =? 0) = true /\
         cycle_count_of_trace t' = 15 + 10 * time_mem + time_branch
     )
-    | 0x80001418 => Some (exists mem gp, s V_MEM32 = Ⓜmem /\ 
+    | 0x80001418 => Some (exists mem, s V_MEM32 = Ⓜmem /\ 
         s R_GP = Ⓓgp /\ s R_SP = Ⓓ(base_sp ⊖ 16) /\
         s R_A1 = Ⓓ(mem Ⓓ[4 + (gp ⊖ 924) ⊕ ((31 ⊖ (clz (uxTopReadyPriority gp mem) 32)) * 20)]) /\
         s R_A2 = Ⓓ(addr_pxReadyTasksLists gp ⊕ ((31 ⊖ (clz (uxTopReadyPriority gp mem) 32)) * 20)) /\
@@ -255,11 +312,16 @@ match t with (Addr a, s) :: t' => match a with
         s R_A4 = Ⓓ(addr_pxReadyTasksLists gp) /\
         s R_A5 = Ⓓ((gp ⊖ 916) ⊕ (31 ⊖ clz (uxTopReadyPriority gp mem) 32) * 20) /\
         common_noverlaps gp base_sp mem /\
-        (uxSchedulerSuspended gp mem =? 0) = true /\
+        uxTopReadyPriority gp mem = uxTopReadyPriority gp base_mem /\
+        mem Ⓓ[(gp ⊖ 920) ⊕ ((31 ⊖ (clz (uxTopReadyPriority gp mem) 32)) * 20)] =
+            base_mem Ⓓ[ 4 + base_mem Ⓓ[(gp ⊖ 920) ⊕ ((31 ⊖ (clz (uxTopReadyPriority gp base_mem) 32)) * 20)]] /\
+        mem Ⓓ[ 4 + mem Ⓓ[ gp ⊖ 920 + (31 ⊖ clz (mem Ⓓ[ gp ⊖ 1920 ]) 32) * 20 ] ] =
+            base_mem Ⓓ[ 4 + base_mem Ⓓ[ gp ⊖ 920 + (31 ⊖ clz (base_mem Ⓓ[ gp ⊖ 1920 ]) 32) * 20 ] ]  /\
+        (uxSchedulerSuspended gp base_mem =? 0) = true /\
         (mem Ⓓ[ 12 + mem Ⓓ[ 48 + pxCurrentTCB gp mem ] ] =?
             mem Ⓓ[ 8 + mem Ⓓ[ 48 + pxCurrentTCB gp mem ] ]) = true /\
         cycle_count_of_trace t' = 36 + clz (mem Ⓓ[ 4294965376 + gp ]) 32 + 2 * time_branch + 14 * time_mem)
-    | 0x80001424 => Some (exists mem' mem gp, s V_MEM32 = Ⓜmem /\
+    (* | 0x80001424 => Some (exists mem' mem, s V_MEM32 = Ⓜmem /\
         s R_GP = Ⓓgp /\ s R_SP = Ⓓ(base_sp ⊖ 16) /\
         (* s R_A1 = Ⓓ(mem Ⓓ[4 + (gp ⊖ 924) ⊕ ((31 ⊖ (clz (uxTopReadyPriority gp mem) 32)) * 20)]) /\ *)
         s R_A2 = Ⓓ(addr_pxReadyTasksLists gp ⊕ ((31 ⊖ (clz (uxTopReadyPriority gp mem) 32)) * 20)) /\
@@ -267,7 +329,10 @@ match t with (Addr a, s) :: t' => match a with
         s R_A4 = Ⓓ(addr_pxReadyTasksLists gp) /\
         (* s R_A5 = Ⓓ((gp ⊖ 916) ⊕ (31 ⊖ clz (uxTopReadyPriority gp mem) 32) * 20) /\ *)
         common_noverlaps gp base_sp mem /\
-        (uxSchedulerSuspended gp mem =? 0) = true /\
+        uxTopReadyPriority gp mem = uxTopReadyPriority gp base_mem /\
+        mem Ⓓ[(gp ⊖ 920) ⊕ ((31 ⊖ (clz (uxTopReadyPriority gp mem) 32)) * 20)] =
+            mem Ⓓ[ 4 + base_mem Ⓓ[ gp ⊖ 920 + (31 ⊖ clz (base_mem Ⓓ[ gp ⊖ 1920 ]) 32) * 20 ] ]  /\
+        (uxSchedulerSuspended gp base_mem =? 0) = true /\
         match (negb (mem' Ⓓ[ 4 + (gp ⊖ 924) ⊕ (31 ⊖ clz (uxTopReadyPriority gp mem') 32) * 20 ] =?
             gp ⊖ 916 ⊕ (31 ⊖ clz (uxTopReadyPriority gp mem') 32) * 20)) with
         | false => mem Ⓓ[(gp ⊖ 920) ⊕ ((31 ⊖ (clz (uxTopReadyPriority gp mem) 32)) * 20)] 
@@ -292,14 +357,11 @@ match t with (Addr a, s) :: t' => match a with
                     time_branch
                 else
                     3 + 2 * time_mem
-            ))
+            )) *)
     | 0x8000138c => Some (
-        exists mem gp, s V_MEM32 = Ⓜmem /\ s R_GP = Ⓓgp /\ 
-        timing_postcondition t gp mem)
+        timing_postcondition t gp base_mem)
     | 0x8000144c => Some (
-        exists mem gp, s V_MEM32 = Ⓜmem /\ s R_GP = Ⓓgp /\
-        (* s R_A5 = Ⓓ(mem Ⓓ[12 + mem Ⓓ[48 + pxCurrentTCB gp mem]]) /\ *)
-        timing_postcondition t gp mem)
+        timing_postcondition t gp base_mem)
     | _ => None end
 | _ => None
 end.
@@ -383,16 +445,13 @@ Theorem vTaskSwitchContext_timing:
          (SP : s R_SP = Ⓓsp)
          (MEM : s V_MEM32 = Ⓜmem)
          (NOVERLAPS : common_noverlaps gp sp mem)
-         (* (GP_SP_FAR : gp_sp_noverlap gp sp)
-         (PCT_NOL_STATIC : pxCurrentTCB_noverlap_static gp mem)
-         (PCT_NOL_SFRAME : pxCurrentTCB_noverlap_stackframe gp sp mem)
-         (MEM_PCT_NOL_SFRAME : mem_pxCurrentTCB_noverlap_stackframe gp sp mem)
-         (MEM_PCT_NOL_STATIC : mem_pxCurrentTCB_noverlap_static gp mem)
-         (SMEM_WELL_FORMED : smem_well_formed gp) *)
+         (MEM4_NOVERLAPS : 
+            mem4_mem4_noverlap_stackframe gp sp mem /\
+            mem4_mem4_noverlap_static gp mem)
          ,
   satisfies_all 
     lifted_vTaskSwitchContext                                 (* Provide lifted code *)
-    (vTaskSwitchContext_timing_invs s p sp)                  (* Provide invariant set *)
+    (vTaskSwitchContext_timing_invs s p sp gp mem)            (* Provide invariant set *)
     vTaskSwitchContext_exit                                   (* Provide exit point *)
   ((x',s')::t).
 Proof using.
@@ -409,13 +468,14 @@ Proof using.
         | [H: common_noverlaps _ _ _ |- _] =>
             destruct H as [GP_SP_FAR [SMEM_WELL_FORMED [PCT_NOL_STATIC 
             [PCT_NOL_SFRAME [PCT_NOL_CLZ [CLZ_NOL_STATIC 
-            [MEM_PCT_NOL_SFRAME [MEM_PCT_NOL_STATIC OFF_MEM_PCT_NOL_CLZ]]]]]]]]
-        end.
+            [MEM_PCT_NOL_SFRAME [MEM_PCT_NOL_STATIC [OFF_MEM_PCT_NOL_CLZ
+            [CLZ_NOL_SFRAME [MEM4_PCT_NOL_SFRAME MEM4_PCT_NOL_STATIC]]]]]]]]]]]
+        end. 
     destruct_noverlaps.
 
     (* Base case *)
     simpl. rewrite ENTRY. step.
-    exists mem, gp. repeat split; try assumption.
+    exists mem. destruct MEM4_NOVERLAPS. repeat split; try assumption.
     unfold uxSchedulerSuspended. unfold msub. psimpl. reflexivity.
 
     (* Inductive step setup *)
@@ -423,114 +483,138 @@ Proof using.
     eapply startof_prefix in ENTRY; try eassumption.
     eapply preservation_exec_prog in MDL; 
         try eassumption; [idtac|apply lift_riscv_welltyped].
-    clear - ENTRY PRE MDL. rename t1 into t. rename s1 into s'.
+    clear - ENTRY PRE MDL. rename t1 into t. rename s1 into s'. 
+    rename mem into base_mem.
 
     (* Meat of proof starts here *)
     destruct_inv 32 PRE.
 
     (* 0x800015e4 *)
-    destruct PRE as [mem [gp [MEM [GP [SP [A4 [NOVERLAPS Cycles]]]]]]].
+    destruct PRE as [mem [MEM [GP [SP [A4 [NOVERLAPS [MEM4_MEM4_NOL_SFRAME
+        [MEM4_MEM4_NOL_STATIC [PreservesPriority [Preserves920 Cycles]]]]]]]]]].
         destruct_noverlaps.
     step. step. step. step. step. step. step. step. step. step.
-    do 2 eexists. repeat split. unfold msub. now psimpl.
+    handle_ex. unfold msub. now psimpl.
         {
-            noverlap_prepare gp sp.
-            rewrite <- getmem_mod_l with (a := 4294965400 + gp);
-            replace (4294965400 ⊕ gp) with (gp ⊖ 1896) by 
-                (unfold msub; psimpl; lia).
-            memsolve mem gp sp; 
-            try solve [ now (
-                apply PCT_NOL_STATIC ||
-                apply PCT_NOL_SFRAME
-            )].
+            noverlap_prepare gp sp; memsolve mem gp sp; auto.
             all: apply noverlap_symmetry;
                 (apply noverlap_shrink with (sp ⊖ 16) 16;
                     [ psimpl; lia | apply noverlap_symmetry]);
                 assumption.
-        }
-        {
-            noverlap_prepare gp sp.
-            rewrite <- getmem_mod_l with (a := 4294965400 + gp);
-            replace (4294965400 ⊕ gp) with (gp ⊖ 1896) by 
-                (unfold msub; psimpl; lia).
-            memsolve mem gp sp;
-            try solve [ now (
-                apply PCT_NOL_STATIC ||
-                apply PCT_NOL_SFRAME ||
-                apply MEM_PCT_NOL_STATIC
-            )].
+        } {
+            noverlap_prepare gp sp; memsolve mem gp sp; auto.
             all: try solve [apply noverlap_symmetry;
                 (apply noverlap_shrink with (sp ⊖ 16) 16;
                     [ psimpl; lia | apply noverlap_symmetry]);
                 assumption].
-        } assumption. assumption.
-        {
+        } {
             unfold pxCurrentTCB_noverlap_static in *.
-            intros. noverlap_prepare gp sp. memsolve mem gp sp.
-            apply PCT_NOL_STATIC, H.
-        }
-        {
+            intros. noverlap_prepare gp sp. memsolve mem gp sp; auto.
+        } {
             unfold pxCurrentTCB_noverlap_stackframe in *.
-            intros. noverlap_prepare gp sp. memsolve mem gp sp.
-            apply PCT_NOL_SFRAME.
-        }
-        {
+            intros. noverlap_prepare gp sp. memsolve mem gp sp; auto.
+        } {
             unfold pxCurrentTCB_noverlap_clz_static in *.
-            noverlap_prepare gp sp; memsolve mem gp sp.
-            assumption.
-        }
-        {
+            noverlap_prepare gp sp; memsolve mem gp sp; auto.
+        } {
             unfold clz_noverlap_smem in *. intros.
             noverlap_prepare gp sp; memsolve mem gp sp.
-            eapply CLZ_NOL_STATIC. eassumption.
-        }
-        {
+            eapply CLZ_NOL_STATIC; eassumption.
+        } {
             unfold mem_pxCurrentTCB_noverlap_stackframe in *.
-            intros. noverlap_prepare gp sp. memsolve mem gp sp.
-                apply MEM_PCT_NOL_SFRAME.
-                now apply PCT_NOL_STATIC.
-                all: apply noverlap_symmetry, noverlap_shrink with (sp ⊖ 16) 16;
-                    [ psimpl; lia |
-                      apply noverlap_symmetry, PCT_NOL_SFRAME ].
-        }
-        {
+            noverlap_prepare gp sp; memsolve mem gp sp; auto.
+            all: apply noverlap_symmetry, noverlap_shrink with (sp ⊖ 16) 16;
+                [ psimpl; lia |
+                    apply noverlap_symmetry, PCT_NOL_SFRAME ].
+        } {
             unfold mem_pxCurrentTCB_noverlap_static in *.
-            intros. noverlap_prepare gp sp. memsolve mem gp sp.
-                now apply MEM_PCT_NOL_STATIC.
-                now apply PCT_NOL_STATIC.
-                all: apply noverlap_symmetry, noverlap_shrink with (sp ⊖ 16) 16;
-                    [ psimpl; lia |
-                      apply noverlap_symmetry, PCT_NOL_SFRAME ].
+            intros. noverlap_prepare gp sp. memsolve mem gp sp; auto.
+            all: apply noverlap_symmetry, noverlap_shrink with (sp ⊖ 16) 16;
+                [ psimpl; lia |
+                    apply noverlap_symmetry, PCT_NOL_SFRAME ].
         } {
             unfold offset_mem_pxCurrentTCB_noverlap_clz. intros.
-            noverlap_prepare gp sp. memsolve mem gp sp.
-                now apply OFF_MEM_PCT_NOL_CLZ.
-            now apply PCT_NOL_STATIC.
+            noverlap_prepare gp sp. memsolve mem gp sp; auto.
             all: apply noverlap_symmetry, noverlap_shrink with (sp ⊖ 16) 16;
                     [ psimpl; lia |
                       apply noverlap_symmetry, PCT_NOL_SFRAME ].
-        }
-        { noverlap_prepare gp sp. memsolve mem gp sp. assumption. }
+        } {
+            unfold clz_noverlap_sframe. 
+            noverlap_prepare gp sp; memsolve mem gp sp; auto.
+        } {
+            unfold mem4_pxCurrentTCB_noverlap_stackframe. intros.
+            noverlap_prepare gp sp; memsolve mem gp sp; auto.
+            apply noverlap_symmetry. auto.
+            apply noverlap_symmetry.
+            apply noverlap_shrink with (sp ⊖ 16) 16.
+                psimpl. lia.
+                auto.
+            apply noverlap_symmetry.
+            apply noverlap_shrink with (sp ⊖ 16) 16.
+                psimpl. lia.
+                auto.
+        } {
+            unfold mem4_pxCurrentTCB_noverlap_static. intros.
+            noverlap_prepare gp sp; memsolve mem gp sp; auto.
+            eapply MEM4_PCT_NOL_STATIC; eassumption.
+            now eapply noverlap_symmetry, CLZ_NOL_STATIC.
+            all: apply noverlap_symmetry, noverlap_shrink with (sp ⊖ 16) 16; [
+                psimpl; lia | auto
+            ]; apply noverlap_symmetry, PCT_NOL_SFRAME.
+        } {
+            unfold mem4_mem4_noverlap_stackframe.
+            noverlap_prepare gp sp; memsolve mem gp sp; auto.
+            all: apply noverlap_symmetry; eauto.
+            all: try solve [
+                apply noverlap_shrink with (sp ⊖ 16) 16;
+                [psimpl;lia|eauto]
+            ].
+            now eapply MEM4_PCT_NOL_STATIC.
+        } {
+            unfold mem4_mem4_noverlap_static. intros.
+            noverlap_prepare gp sp; memsolve mem gp sp; eauto.
+            all: apply noverlap_symmetry; eauto.
+            all: try solve [
+                apply noverlap_shrink with (sp ⊖ 16) 16;
+                [psimpl;lia|eauto]
+            ].
+            now eapply MEM4_PCT_NOL_STATIC.
+        } {
+            unfold uxTopReadyPriority. 
+            noverlap_prepare gp sp; memsolve mem gp sp; auto.
+        } {
+            noverlap_prepare gp sp.
+            repeat rewrite <- getmem_mod_l with (a := _ + _).
+            rewrite getmem_mod_l.
+            memsolve mem gp sp;
+                try solve [apply noverlap_symmetry; auto].
+            repeat rewrite getmem_mod_l; now rewrite Preserves920.
+            all: try solve [apply noverlap_symmetry, noverlap_shrink with (sp ⊖ 16) 16;
+                [psimpl; lia|auto]].
+            now eapply noverlap_symmetry, MEM4_PCT_NOL_STATIC.
+        } 
         hammer. rewrite A4, BC, Cycles. lia.
-    step. step. handle_ex.
-        unfold timing_postcondition. unfold uxSchedulerSuspended in *.
-            rewrite getmem_frame; try (left; psimpl; lia).
+    step. step.
+        unfold timing_postcondition.
         rewrite BC.
         hammer. rewrite A4, BC, Cycles. lia.
 
     (* 0x800013c8 *)
-    destruct PRE as [mem [gp [MEM [GP [SP [A5 [A2 [A4 [NOVERLAPS [BR0 Cycles]]]]]]]]]].
+    destruct PRE as [mem [MEM [GP [SP [A5 [A2 [A4 [NOVERLAPS [MEM4_MEM4_NOL_SFRAME
+        [MEM4_MEM4_NOL_STATIC [PreservesPriority [Preserves920 [BR0 Cycles]]]]]]]]]]]]]. 
         destruct_noverlaps.
     step.
         step. step. step. step. step. step. step. step. step. step.
         exact I. (* Infinite loop, stack overflow detected *)
-    step. handle_ex. change ((678490 << 12) + 1445) with 0xa5a5a5a5 in *.
+    step. handle_ex.
         now apply Bool.negb_false_iff in BC.
+        change ((678490 << 12) + 1445) with 0xa5a5a5a5 in *.
         hammer. rewrite A2, A4, BC, Cycles. lia.
 
     (* 0x800013d0 *)
-    destruct PRE as [mem [gp [MEM [GP [SP [A2 [A3 [A5 [NOVERLAPS [NotSuspended 
-        [Br Cycles]]]]]]]]]]]. destruct_noverlaps.
+    destruct PRE as [mem [MEM [GP [SP [A2 [A3 [A5 [NOVERLAPS [MEM4_MEM4_NOL_SFRAME
+        [MEM4_MEM4_NOL_STATIC [PreservesPriority [Preserves920 [NotSuspended [Br Cycles]]]]]]]]]]]]]]. 
+    destruct_noverlaps.
     step.
         step. step. step. step. step. step. step. step. step. step.
         exact I. (* Infinite loop, stack overflow detected *)
@@ -539,8 +623,9 @@ Proof using.
         hammer. rewrite A2, A3, Cycles, BC. lia.
 
     (* 0x800013d8 *)
-    destruct PRE as [mem [gp [MEM [GP [SP [A3 [A4 [A5 [NOVERLAPS
-        [B1 [B2 [NotSuspended Cycles]]]]]]]]]]]]. destruct_noverlaps.
+    destruct PRE as [mem [MEM [GP [SP [A3 [A4 [A5 [NOVERLAPS [MEM4_MEM4_NOL_SFRAME
+        [MEM4_MEM4_NOL_STATIC [PreservesPriority [Preserves920 [B1 [B2 
+        [NotSuspended Cycles]]]]]]]]]]]]]]]. destruct_noverlaps.
     step.
         step. step. step. step. step. step. step. step. step. step.
         exact I. (* Infinite loop, stack overflow detected *)
@@ -550,463 +635,150 @@ Proof using.
         hammer. rewrite A3, A4, BC, Cycles. lia.
 
     (* 0x800013e0 *)
-    destruct PRE as [mem [gp [MEM [GP [SP [A3 [A4 [A5 [NOVERLAPS [B1 [B2 [B3 
-        [NotSuspended Cycles]]]]]]]]]]]]]. destruct_noverlaps.
+    destruct PRE as [mem [MEM [GP [SP [A3 [A4 [A5 [NOVERLAPS [MEM4_MEM4_NOL_SFRAME 
+        [MEM4_MEM4_NOL_STATIC [PreservesPriority [Preserves920 [B1 [B2 [B3 
+        [NotSuspended Cycles]]]]]]]]]]]]]]]]. destruct_noverlaps.
     step. step. step. step. step. step. step. step. step. step. step.
     step. step. step. step.
         handle_ex.
         {
             unfold uxTopReadyPriority.
             noverlap_prepare gp sp.
-            rewrite <- getmem_mod_l with (a := 4294965376 + gp);
-            replace (4294965376 ⊕ gp) with (gp ⊖ 1920) by 
-                (unfold msub; psimpl; lia).
-            rewrite <- getmem_mod_l with (a := 4294966376 + gp + 
-                (31 ⊖ clz (mem Ⓓ[ gp ⊖ 1920 ]) 32) * 20).
-            replace (mem Ⓓ[ 4294966376 + gp ⊕ (31 ⊖ clz (mem Ⓓ[ gp ⊖ 1920 ]) 32) * 20 ])
-            with (mem Ⓓ[ gp ⊖ 920 ⊕ (31 ⊖ clz (mem Ⓓ[ gp ⊖ 1920 ]) 32) * 20 ]); cycle 7.
-                unfold msub at 1; now psimpl.
-            rewrite <- setmem_mod_l, (N.add_comm 4294966376).
-            assert (forall n, gp + 4294966376 ⊕ n = gp ⊖ 920 ⊕ n). {
-                intros. unfold msub. simpl (_ - _ mod _).
-                now psimpl.
-            } rewrite H. clear H.
-            assert (forall n, 4 + (gp ⊖ 924) ⊕ n = (gp ⊖ 920) ⊕ n).
-                intros; unfold msub; simpl (_ - _ mod _); now psimpl.
-            rewrite H. clear H. psimpl.
             replace (clz
             ((mem [Ⓓgp ⊖ 920 ⊕ (31 ⊖ clz (mem Ⓓ[ gp ⊖ 1920 ]) 32) * 20
               := mem
                  Ⓓ[ 4 + mem Ⓓ[ gp ⊖ 920 ⊕ (31 ⊖ clz (mem Ⓓ[ gp ⊖ 1920 ]) 32) * 20 ]
                  ] ]) Ⓓ[ gp ⊖ 1920 ]) 32) with 
                 (clz (mem Ⓓ[ gp ⊖ 1920 ]) 32); cycle 1. {
-                f_equal. memsolve mem gp sp.
-                apply sep_noverlap; left; psimpl;
-                pose proof (clz_le_w (mem Ⓓ[ gp ⊖ 1920 ]) 32);
-                remember (clz (mem Ⓓ[ gp ⊖ 1920 ]) 32) as n; clear Heqn;
-                do 33 (destruct n as [| n _] using N.peano_ind;
-                    [cbn [N.succ Pos.succ]; psimpl; lia|
-                    replace (N.succ n) with (1 + n) in H by lia; psimpl in H]);
-                lia.
+                f_equal. memsolve mem gp sp; auto.
             } psimpl. reflexivity.
-        }
-        {
+        } {
             unfold addr_pxReadyTasksLists, uxTopReadyPriority.
-            noverlap_prepare gp sp; memsolve mem gp sp. f_equal.
-                unfold msub; psimpl.
-                replace (2 ^ 32 - 1920 mod 2 ^ 32) with 4294965376 by reflexivity.
-                now rewrite getmem_mod_l, (N.add_comm gp).
-            unfold msub at 1; psimpl.
-            apply sep_noverlap; left; psimpl;
-                pose proof (clz_le_w (mem Ⓓ[ 4294965376 + gp ]) 32);
-                remember (clz (mem Ⓓ[ 4294965376 + gp ]) 32) as n; clear Heqn;
-                do 33 (destruct n as [| n _] using N.peano_ind;
-                    [cbn [N.succ Pos.succ]; psimpl; lia|
-                    replace (N.succ n) with (1 + n) in H by lia; psimpl in H]);
-                lia.
-        }
-        {
+            noverlap_prepare gp sp; memsolve mem gp sp; auto.
+        } {
             unfold uxTopReadyPriority.
-            noverlap_prepare gp sp; memsolve mem gp sp.
-                unfold msub at 3. simpl (_ - _ mod _).
-                now rewrite getmem_mod_l, (N.add_comm 4294965376).
-            apply sep_noverlap; left; psimpl;
-                pose proof (clz_le_w (mem Ⓓ[ 4294965376 + gp ]) 32);
-                remember (clz (mem Ⓓ[ 4294965376 + gp ]) 32) as n; clear Heqn;
-                do 33 (destruct n as [| n _] using N.peano_ind;
-                    [cbn [N.succ Pos.succ]; psimpl; lia|
-                    replace (N.succ n) with (1 + n) in H by lia; psimpl in H]);
-                lia.
+            noverlap_prepare gp sp; memsolve mem gp sp; auto.
         }
         now unfold addr_pxReadyTasksLists, msub; psimpl.
         {
             unfold uxTopReadyPriority.
-            noverlap_prepare gp sp; memsolve mem gp sp. f_equal.
-                unfold msub at 2 4. simpl (_ - _ mod _).
-                rewrite N.add_comm, N.add_assoc.
-                rewrite (N.add_comm _ gp), getmem_mod_l. now psimpl.
-            apply sep_noverlap; left; psimpl;
-                pose proof (clz_le_w (mem Ⓓ[ 4294965376 + gp ]) 32);
-                remember (clz (mem Ⓓ[ 4294965376 + gp ]) 32) as n; clear Heqn;
-                do 33 (destruct n as [| n _] using N.peano_ind;
-                    [cbn [N.succ Pos.succ]; psimpl; lia|
-                    replace (N.succ n) with (1 + n) in H by lia; psimpl in H]);
-                lia.
-        }
-        {
+            noverlap_prepare gp sp; memsolve mem gp sp; auto. f_equal.
+            unfold msub; psimpl; simpl (2^32 - _ mod _).
+                now rewrite N.add_comm, N.add_assoc,
+                    (N.add_comm _ gp), getmem_mod_l.
+        } {
             unfold pxCurrentTCB_noverlap_static. intros.
-            noverlap_prepare gp sp; memsolve mem gp sp.
-            now apply PCT_NOL_STATIC.
-            unfold msub at 1. simpl (_ - _ mod _).
-            apply sep_noverlap; left; psimpl;
-                pose proof (clz_le_w (mem Ⓓ[ 4294965376 + gp ]) 32);
-                remember (clz (mem Ⓓ[ 4294965376 + gp ]) 32) as n; clear Heqn;
-                do 33 (destruct n as [| n _] using N.peano_ind;
-                    [cbn [N.succ Pos.succ]; psimpl; lia|
-                    replace (N.succ n) with (1 + n) in H by lia; psimpl in H]);
-                lia.
-        }
-        {
-            unfold pxCurrentTCB_noverlap_stackframe. intros.
-            noverlap_prepare gp sp; memsolve mem gp sp.
-            now apply PCT_NOL_SFRAME.
-            unfold msub at 1. simpl (_ - _ mod _).
-            apply sep_noverlap; left; psimpl;
-                pose proof (clz_le_w (mem Ⓓ[ 4294965376 + gp ]) 32);
-                remember (clz (mem Ⓓ[ 4294965376 + gp ]) 32) as n; clear Heqn;
-                do 33 (destruct n as [| n _] using N.peano_ind;
-                    [cbn [N.succ Pos.succ]; psimpl; lia|
-                    replace (N.succ n) with (1 + n) in H by lia; psimpl in H]);
-                lia.
-        }
-        {
+            noverlap_prepare gp sp; memsolve mem gp sp; auto.
+        } {
+            unfold pxCurrentTCB_noverlap_stackframe.
+            noverlap_prepare gp sp; memsolve mem gp sp; auto.
+        } {
             unfold pxCurrentTCB_noverlap_clz_static.
-            noverlap_prepare gp sp; memsolve mem gp sp.
-            now apply PCT_NOL_CLZ.
-            all: unfold msub at 1; simpl (_ - _ mod _);
-            apply sep_noverlap; left; psimpl;
-                pose proof (clz_le_w (mem Ⓓ[ 4294965376 + gp ]) 32);
-                remember (clz (mem Ⓓ[ 4294965376 + gp ]) 32) as n; clear Heqn;
-                do 33 (destruct n as [| n _] using N.peano_ind;
-                    [cbn [N.succ Pos.succ]; psimpl; lia|
-                    replace (N.succ n) with (1 + n) in H by lia; psimpl in H]);
-                lia.
-        }
-        {
-            unfold clz_noverlap_smem in *. intros.
-            replace ((mem
-            [Ⓓ4294966376 + gp + (31 ⊖ clz (mem Ⓓ[ 4294965376 + gp ]) 32) * 20
+            noverlap_prepare gp sp; memsolve mem gp sp; auto.
+        } {
+            unfold clz_noverlap_smem. intros.
+            noverlap_prepare gp sp.
+            replace ((mem [Ⓓgp ⊖ 920 ⊕ (31 ⊖ clz (mem Ⓓ[ gp ⊖ 1920 ]) 32) * 20
             := mem
                Ⓓ[ 4 +
-                  mem
-                  Ⓓ[ 4294966376 + gp +
-                     (31 ⊖ clz (mem Ⓓ[ 4294965376 + gp ]) 32) * 20 ] ] ])
-           Ⓓ[ gp ⊖ 1920 ]) with (mem Ⓓ[gp ⊖ 1920]).
-           eapply CLZ_NOL_STATIC. eassumption.
-           rewrite <- setmem_mod_l.
-           rewrite <- getmem_mod_l with (a := 4294966376 + gp + (31 ⊖ clz (mem Ⓓ[ 4294965376 + gp ]) 32) * 20).
-           rewrite getmem_noverlap. reflexivity.
-           rewrite <- getmem_mod_l. 
-           replace (mem Ⓓ[ 4294965376 ⊕ gp ]) with (mem Ⓓ[ gp ⊖ 1920 ]) by (unfold msub; psimpl; lia).
-           replace (4294966376 + gp ⊕ (31 ⊖ clz (mem Ⓓ[ gp ⊖ 1920 ]) 32) * 20) with
-                (gp ⊖ 920 ⊕ (31 ⊖ clz (mem Ⓓ[ gp ⊖ 1920 ]) 32) * 20).
-           now eapply CLZ_NOL_STATIC.
-           now unfold msub at 1; psimpl.
-        }
-        {
+                  mem Ⓓ[ gp ⊖ 920 ⊕ (31 ⊖ clz (mem Ⓓ[ gp ⊖ 1920 ]) 32) * 20 ]
+               ] ]) Ⓓ[ gp ⊖ 1920 ]) with (mem Ⓓ[gp ⊖ 1920]) by
+               (rewrite getmem_noverlap; auto).
+           eapply CLZ_NOL_STATIC; eassumption.
+        } {
             unfold mem_pxCurrentTCB_noverlap_stackframe.
-            replace (mem Ⓓ[ 4294966376 + gp + (31 ⊖ clz (mem Ⓓ[ 4294965376 + gp ]) 32) * 20 ])
-                with (mem Ⓓ[ (gp ⊖ 920) + (31 ⊖ clz (mem Ⓓ[ gp ⊖ 1920 ]) 32) * 20 ]).
-            replace (mem [Ⓓ4294966376 + gp + (31 ⊖ clz (mem Ⓓ[ 4294965376 + gp ]) 32) * 20
-                := mem Ⓓ[ 4 + mem Ⓓ[ gp ⊖ 920 + (31 ⊖ clz (mem Ⓓ[ gp ⊖ 1920 ]) 32) * 20 ]]])
-                with (mem [Ⓓ(gp ⊖ 920) + (31 ⊖ clz (mem Ⓓ[ 4294965376 + gp ]) 32) * 20
-                := mem Ⓓ[ 4 + mem Ⓓ[ gp ⊖ 920 + (31 ⊖ clz (mem Ⓓ[ gp ⊖ 1920 ]) 32) * 20 ]]]).
-            rewrite <- setmem_mod_l.
-            noverlap_prepare gp sp; memsolve mem gp sp.
-            now apply MEM_PCT_NOL_SFRAME.
-            all: try solve [unfold msub at 1; simpl (_ - _ mod _);
-                apply sep_noverlap; left; psimpl;
-                pose proof (clz_le_w (mem Ⓓ[ 4294965376 + gp ]) 32);
-                remember (clz (mem Ⓓ[ 4294965376 + gp ]) 32) as n; clear Heqn;
-                do 33 (destruct n as [| n _] using N.peano_ind;
-                    [cbn [N.succ Pos.succ]; psimpl; lia|
-                    replace (N.succ n) with (1 + n) in H by lia; psimpl in H]);
-                lia].
-            replace (mem Ⓓ[ 4294965376 + gp ]) with (mem Ⓓ[gp ⊖ 1920]) by 
-                (unfold msub; simpl (_ - _ mod _); psimpl; lia).
-            apply PCT_NOL_CLZ.
-            unfold msub at 1. simpl (_ - _ mod _).
-                rewrite <- setmem_mod_l with 
-                    (a := gp ⊕ 4294966376 + (31 ⊖ clz (mem Ⓓ[ 4294965376 + gp ]) 32) * 20).
-                rewrite <- setmem_mod_l with
-                    (a := 4294966376 + gp + (31 ⊖ clz (mem Ⓓ[ 4294965376 + gp ]) 32) * 20).
-                now psimpl.
-            unfold msub at 1 3; simpl (_ - _ mod _).
-                rewrite getmem_mod_l; psimpl.
-                now rewrite (N.add_comm gp).
-        }
-        {
+            noverlap_prepare gp sp; memsolve mem gp sp; auto.
+        } {
             unfold mem_pxCurrentTCB_noverlap_static. intros.
-            noverlap_prepare gp sp.
-            rewrite <- getmem_mod_l with (a := 4294965376 + gp);
-            replace (4294965376 ⊕ gp) with (gp ⊖ 1920) by 
-                (unfold msub; psimpl; lia).
-            rewrite <- getmem_mod_l with (a := 4294966376 + gp + 
-                (31 ⊖ clz (mem Ⓓ[ gp ⊖ 1920 ]) 32) * 20).
-            replace (mem Ⓓ[ 4294966376 + gp ⊕ (31 ⊖ clz (mem Ⓓ[ gp ⊖ 1920 ]) 32) * 20 ])
-            with (mem Ⓓ[ gp ⊖ 920 ⊕ (31 ⊖ clz (mem Ⓓ[ gp ⊖ 1920 ]) 32) * 20 ]); cycle 7.
-                unfold msub at 1; now psimpl.
-            rewrite <- setmem_mod_l, (N.add_comm 4294966376).
-            assert (forall n, gp + 4294966376 ⊕ n = gp ⊖ 920 ⊕ n).
-                intros; unfold msub; simpl (_ - _ mod _);
-                now psimpl.
-            rewrite H0. clear H0. psimpl.
-            replace ((mem [Ⓓgp ⊖ 920 + (31 ⊖ clz (mem Ⓓ[ gp ⊖ 1920 ]) 32) * 20
-                := mem Ⓓ[ 4 + mem Ⓓ[ gp ⊖ 920 + (31 ⊖ clz (mem Ⓓ[ gp ⊖ 1920 ]) 32) * 20 ] ] ])
-            Ⓓ[ 48 +
-                (mem [Ⓓgp ⊖ 920 + (31 ⊖ clz (mem Ⓓ[ gp ⊖ 1920 ]) 32) * 20
-                := mem Ⓓ[ 4 + mem Ⓓ[ gp ⊖ 920 + (31 ⊖ clz (mem Ⓓ[ gp ⊖ 1920 ]) 32) * 20 ] ] ])
-                Ⓓ[ gp ⊖ 1896 ] ]) with (mem Ⓓ[48 + pxCurrentTCB gp mem]).
-            now apply MEM_PCT_NOL_STATIC.
-            rewrite <- setmem_mod_l with (a := gp ⊖ 920 + (31 ⊖ clz (mem Ⓓ[ gp ⊖ 1920 ]) 32) * 20).
-            memsolve mem gp sp. reflexivity.
-            (* unfold msub at 1 4; simpl (_ - _ mod _). *)
-            all: try solve [unfold msub at 1 4; simpl (_ - _ mod _);
-                apply sep_noverlap; left; psimpl;
-                pose proof (clz_le_w (mem Ⓓ[ gp ⊕ 4294965376 ]) 32);
-                remember (clz (mem Ⓓ[ gp ⊕ 4294965376 ]) 32) as n; clear Heqn;
-                do 33 (destruct n as [| n _] using N.peano_ind;
-                    [cbn [N.succ Pos.succ]; psimpl; lia|
-                    replace (N.succ n) with (1 + n) in H by lia; psimpl in H]);
-                lia].
-            assumption.
+            noverlap_prepare gp sp; memsolve mem gp sp; auto.
         } {
             unfold offset_mem_pxCurrentTCB_noverlap_clz. intros.
-            noverlap_prepare gp sp. rewrite <- setmem_mod_l.
-            memsolve mem gp sp;
-                try replace (4294966376 + gp ⊕ (31 ⊖ clz (mem Ⓓ[ 4294965376 + gp ]) 32) * 20) with
-                    (gp ⊖ 920 ⊕ (31 ⊖ clz (mem Ⓓ[ 4294965376 + gp ]) 32) * 20) by 
-                    (unfold msub; now psimpl);
-                replace (mem Ⓓ[ 4294965376 + gp ]) with (mem Ⓓ[ gp ⊖ 1920 ]) by
-                    (unfold msub; now psimpl).
-                now apply OFF_MEM_PCT_NOL_CLZ.
-            all: try now apply CLZ_NOL_STATIC.
-            apply PCT_NOL_CLZ.
-        }
-        {
-            noverlap_prepare gp sp; memsolve mem gp sp.
-            assumption.
-            apply sep_noverlap; left; psimpl;
-                pose proof (clz_le_w (mem Ⓓ[ 4294965376 + gp ]) 32);
-                remember (clz (mem Ⓓ[ 4294965376 + gp ]) 32) as n; clear Heqn;
-                do 33 (destruct n as [| n _] using N.peano_ind;
-                    [cbn [N.succ Pos.succ]; psimpl; lia|
-                    replace (N.succ n) with (1 + n) in H by lia; psimpl in H]);
-                lia.
+            noverlap_prepare gp sp; memsolve mem gp sp; auto.
         } {
-            rewrite <- setmem_mod_l.
+            unfold clz_noverlap_sframe.
+            noverlap_prepare gp sp; memsolve mem gp sp; auto.
+        } {
+            unfold mem4_pxCurrentTCB_noverlap_stackframe.
             noverlap_prepare gp sp.
-            memsolve mem gp sp;
-                try replace (4294966376 + gp ⊕ (31 ⊖ clz (mem Ⓓ[ 4294965376 + gp ]) 32) * 20) with
-                    (gp ⊖ 920 ⊕ (31 ⊖ clz (mem Ⓓ[ 4294965376 + gp ]) 32) * 20) by 
-                    (unfold msub; now psimpl);
-                replace (mem Ⓓ[ 4294965376 + gp ]) with (mem Ⓓ[ gp ⊖ 1920 ]) by
-                    (unfold msub; now psimpl); auto.
+            replace (clz ((mem [Ⓓ_ := _ ]) Ⓓ[ gp ⊖ 1920 ]) 32) 
+                with (clz (mem Ⓓ[ gp ⊖ 1920 ]) 32) by
+                (f_equal; rewrite getmem_noverlap; auto).
+            psimpl.
+            rewrite <- getmem_mod_l with (a := gp ⊖ _ + _).
+            eapply MEM4_MEM4_NOL_SFRAME.
+        } {
+            unfold mem4_pxCurrentTCB_noverlap_static. intros.
+            noverlap_prepare gp sp.
+            replace (clz ((mem [Ⓓ_ := _ ]) Ⓓ[ gp ⊖ 1920 ]) 32) 
+                with (clz (mem Ⓓ[ gp ⊖ 1920 ]) 32) by
+                (f_equal; rewrite getmem_noverlap; auto).
+            psimpl.
+            rewrite <- getmem_mod_l with (a := gp ⊖ _ + _).
+            eapply MEM4_MEM4_NOL_STATIC; eassumption.
+        } {
+            unfold uxTopReadyPriority.
+            noverlap_prepare gp sp; memsolve mem gp sp; auto.
+        } {
+            unfold uxTopReadyPriority in *.
+            noverlap_prepare gp sp.
+            replace (clz ((mem [Ⓓ_ := _ ]) Ⓓ[ gp ⊖ 1920 ]) 32) 
+                with (clz (mem Ⓓ[ gp ⊖ 1920 ]) 32) by
+                (f_equal; rewrite getmem_noverlap; auto).
+            psimpl. now rewrite Preserves920.
+        } { noverlap_prepare gp sp.
+            replace (clz ((mem [Ⓓ_ := _ ]) Ⓓ[ gp ⊖ 1920 ]) 32) 
+                with (clz (mem Ⓓ[ gp ⊖ 1920 ]) 32) by
+                (f_equal; rewrite getmem_noverlap; auto).
+            psimpl.
+            rewrite <- Preserves920.
+            admit. (* True because both overlapping and non-overlapping are true *) 
+            (* Actually because addrs might not be byte-aligned, need another 
+            noverlap assumption? *)
+        } { 
+            noverlap_prepare gp sp; memsolve mem gp sp; auto.
         }
         hammer. rewrite A4, A5, BC, Cycles. psimpl.
-        (* Can't infer placeholder? *)
-        replace ((mem[Ⓓ4294966376 + gp + (31 ⊖ clz (mem Ⓓ[ 4294965376 + gp ]) 32) * 20
-                    := mem Ⓓ[ 4 + mem Ⓓ[ 4294966376 + gp + 
-                                (31 ⊖ clz (mem Ⓓ[ 4294965376 + gp ]) 32) * 20 ]
-                            ] 
-                    ]) Ⓓ[ 4294965376 + gp ]) with (mem Ⓓ[ 4294965376 + gp ]).
+        noverlap_prepare gp sp.
+        replace (clz ((mem [Ⓓ_ := _ ]) Ⓓ[ gp ⊖ 1920 ]) 32) 
+                with (clz (mem Ⓓ[ gp ⊖ 1920 ]) 32) by
+                (f_equal; rewrite getmem_noverlap; auto).
         lia.
-        {
-            noverlap_prepare gp sp. memsolve mem gp sp.
-            apply sep_noverlap; left; psimpl;
-                pose proof (clz_le_w (mem Ⓓ[ 4294965376 + gp ]) 32);
-                remember (clz (mem Ⓓ[ 4294965376 + gp ]) 32) as n; clear Heqn;
-                do 33 (destruct n as [| n _] using N.peano_ind;
-                    [cbn [N.succ Pos.succ]; psimpl; lia|
-                    replace (N.succ n) with (1 + n) in H by lia; psimpl in H]);
-                lia.
-        }
     (* Inside vApplicationStackOverflowHook *)
     step. step. step. step. step. step. step. step. step. step. exact I.
 
-    (* 0x80001418 *)
-    destruct PRE as [mem [gp [MEM [GP [SP [A1 [A2 [A3 [A4 [A5 [NOVERLAPS 
-        [NotSuspended [B1 Cycles]]]]]]]]]]]]]. destruct_noverlaps.
-    rename mem into mem'.
-    step.
-        exists mem'. handle_ex.
-            now rewrite BC.
-        hammer. rewrite getmem_mod_l, <- getmem_mod_l with (a := _ + _ + _).
-        replace ((gp ⊖ 916 + (31 ⊖ clz (uxTopReadyPriority gp mem') 32) * 20) mod 4294967296)
-            with ((gp ⊖ 916 ⊕ (31 ⊖ clz (uxTopReadyPriority gp mem') 32) * 20)) by reflexivity.
-        rewrite A1, A5, BC.
-        rewrite Cycles. lia.
-    step. step.
-        exists mem'. handle_ex.
-        {
-            unfold uxTopReadyPriority, addr_pxReadyTasksLists.
-            rewrite <- setmem_mod_l.
-            memsolve mem' gp sp.
-            replace (4 + (gp ⊖ 924) ⊕ (31 ⊖ clz (mem' Ⓓ[ gp ⊖ 1920 ]) 32) * 20) with
-                ((gp ⊖ 920) ⊕ (31 ⊖ clz (mem' Ⓓ[ gp ⊖ 1920 ]) 32) * 20) by
-                (unfold msub; now psimpl).
-            now apply CLZ_NOL_STATIC.
-        } {
-            unfold uxTopReadyPriority, addr_pxReadyTasksLists.
-            rewrite <- setmem_mod_l.
-            memsolve mem' gp sp. assumption.
-            replace (4 + (gp ⊖ 924) ⊕ (31 ⊖ clz (mem' Ⓓ[ gp ⊖ 1920 ]) 32) * 20) with
-                ((gp ⊖ 920) ⊕ (31 ⊖ clz (mem' Ⓓ[ gp ⊖ 1920 ]) 32) * 20) by
-                (unfold msub; now psimpl).
-            now apply CLZ_NOL_STATIC.
-        } {
-            unfold pxCurrentTCB_noverlap_static, 
-                addr_pxReadyTasksLists, uxTopReadyPriority, pxCurrentTCB. intros.
-            rewrite <- setmem_mod_l.
-            memsolve mem' gp sp. now apply PCT_NOL_STATIC.
-            replace (4 + _ ⊕ _) with ((gp ⊖ 920) ⊕ (31 ⊖ clz (mem' Ⓓ[ gp ⊖ 1920 ]) 32) * 20)
-                by (unfold msub; now psimpl).
-            now apply CLZ_NOL_STATIC.
-        } {
-            unfold pxCurrentTCB_noverlap_stackframe, 
-                addr_pxReadyTasksLists, uxTopReadyPriority, pxCurrentTCB. intros.
-            rewrite <- setmem_mod_l.
-            memsolve mem' gp sp. apply PCT_NOL_SFRAME.
-            replace (4 + _ ⊕ _) with ((gp ⊖ 920) ⊕ (31 ⊖ clz (mem' Ⓓ[ gp ⊖ 1920 ]) 32) * 20)
-                by (unfold msub; now psimpl).
-            now apply CLZ_NOL_STATIC.
-        } {
-            unfold pxCurrentTCB_noverlap_clz_static, 
-                addr_pxReadyTasksLists, uxTopReadyPriority, pxCurrentTCB. intros.
-            rewrite <- setmem_mod_l.
-            memsolve mem' gp sp;
-                try replace (4 + _ ⊕ _) with ((gp ⊖ 920) ⊕ (31 ⊖ clz (mem' Ⓓ[ gp ⊖ 1920 ]) 32) * 20)
-                    by (unfold msub; now psimpl).
-            apply PCT_NOL_CLZ.
-            now apply CLZ_NOL_STATIC.
-            now apply CLZ_NOL_STATIC.
-        } {
-            unfold clz_noverlap_smem, 
-                addr_pxReadyTasksLists, uxTopReadyPriority, pxCurrentTCB. intros.
-            rewrite <- setmem_mod_l.
-            memsolve mem' gp sp;
-                try replace (4 + _ ⊕ _) with ((gp ⊖ 920) ⊕ (31 ⊖ clz (mem' Ⓓ[ gp ⊖ 1920 ]) 32) * 20)
-                    by (unfold msub; now psimpl).
-            now apply CLZ_NOL_STATIC.
-            now apply CLZ_NOL_STATIC.
-        } {
-            unfold mem_pxCurrentTCB_noverlap_stackframe, 
-                addr_pxReadyTasksLists, uxTopReadyPriority, pxCurrentTCB. intros.
-            rewrite <- setmem_mod_l.
-            memsolve mem' gp sp;
-                try replace (4 + _ ⊕ _) with ((gp ⊖ 920) ⊕ (31 ⊖ clz (mem' Ⓓ[ gp ⊖ 1920 ]) 32) * 20)
-                    by (unfold msub; now psimpl).
-            apply MEM_PCT_NOL_SFRAME.
-            now apply CLZ_NOL_STATIC.
-            apply PCT_NOL_CLZ.
-            now apply CLZ_NOL_STATIC.
-        } {
-            unfold mem_pxCurrentTCB_noverlap_static, 
-                addr_pxReadyTasksLists, uxTopReadyPriority, pxCurrentTCB. intros.
-            rewrite <- setmem_mod_l.
-            memsolve mem' gp sp;
-                try replace (4 + _ ⊕ _) with ((gp ⊖ 920) ⊕ (31 ⊖ clz (mem' Ⓓ[ gp ⊖ 1920 ]) 32) * 20)
-                    by (unfold msub; now psimpl).
-            now apply MEM_PCT_NOL_STATIC.
-            now apply CLZ_NOL_STATIC.
-            apply PCT_NOL_CLZ.
-            now apply CLZ_NOL_STATIC.
-        } {
-            unfold offset_mem_pxCurrentTCB_noverlap_clz, addr_pxReadyTasksLists,
-                uxTopReadyPriority, pxCurrentTCB. intros.
-            rewrite <- setmem_mod_l.
-            memsolve mem' gp sp;
-                try replace (4 + _ ⊕ _) with ((gp ⊖ 920) ⊕ (31 ⊖ clz (mem' Ⓓ[ gp ⊖ 1920 ]) 32) * 20)
-                    by (unfold msub; now psimpl); auto.
-        } {
-            unfold uxSchedulerSuspended, 
-                addr_pxReadyTasksLists, uxTopReadyPriority, pxCurrentTCB.
-            rewrite <- setmem_mod_l.
-            memsolve mem' gp sp;
-                try replace (4 + _ ⊕ _) with ((gp ⊖ 920) ⊕ (31 ⊖ clz (mem' Ⓓ[ gp ⊖ 1920 ]) 32) * 20)
-                    by (unfold msub; now psimpl).
-            assumption.
-            now apply CLZ_NOL_STATIC.
-        } {
-            rewrite BC.
-            rewrite <- setmem_mod_l, <- getmem_mod_l with (a := _ + _ + _).
-            unfold addr_pxReadyTasksLists, uxTopReadyPriority. psimpl.
-            unfold msub at 5. psimpl.
-            replace ((mem' [Ⓓ4 + (gp ⊖ 924) ⊕ (31 ⊖ clz (mem' Ⓓ[ gp ⊖ 1920 ]) 32) * 20
-                := mem' Ⓓ[ 12 + (gp ⊖ 924) ⊕ (31 ⊖ clz (mem' Ⓓ[ gp ⊖ 1920 ]) 32) * 20 ] ])
-                Ⓓ[ gp ⊖ 1920 ]) with (mem' Ⓓ[ gp ⊖ 1920 ]).
-            psimpl. repeat split. 
-                unfold msub; now psimpl. 
-                apply Bool.negb_false_iff, N.eqb_eq in BC. unfold uxTopReadyPriority in BC. 
-                    rewrite <- BC. unfold msub; now psimpl.
-                rewrite getmem_mod_l.
-                replace (4294966384 + gp ⊕ (31 ⊕ (2 ^ 32 - clz (mem' Ⓓ[ gp ⊕ (2 ^ 32 - 1920 mod 2 ^ 32) ]) 32 mod 2 ^ 32)) * 20)
-                with (gp ⊖ 912 ⊕ (31 ⊕ (2 ^ 32 - clz (mem' Ⓓ[ gp ⊕ (2 ^ 32 - 1920 mod 2 ^ 32) ]) 32 mod 2 ^ 32)) * 20).
-                replace (gp ⊕ (2 ^ 32 - 916 mod 2 ^ 32)) with (gp ⊖ 916) by (unfold msub; now psimpl).
-            rewrite getmem_noverlap. reflexivity.
-            replace (4 + _ ⊕ _) with ((gp ⊖ 920) ⊕ (31 ⊖ clz (mem' Ⓓ[ gp ⊖ 1920 ]) 32) * 20)
-                by (unfold msub; now psimpl).
-            now apply CLZ_NOL_STATIC.
-            unfold msub. now psimpl.
-        }
-        hammer. rewrite A1, A5, BC, Cycles. rewrite getmem_mod_l in *.
-        replace ((gp ⊖ 916 + (31 ⊖ clz (uxTopReadyPriority gp mem') 32) * 20) mod 4294967296)
-            with ((gp ⊖ 916 ⊕ (31 ⊖ clz (uxTopReadyPriority gp mem') 32) * 20)) by reflexivity.
-        rewrite BC.
-        replace ((mem' [Ⓓ4 + addr_pxReadyTasksLists gp + (31 ⊖ clz (uxTopReadyPriority gp mem') 32) * 20
-            := mem' Ⓓ[ 12 + addr_pxReadyTasksLists gp +
-                (31 ⊖ clz (uxTopReadyPriority gp mem') 32) * 20 ] ]) Ⓓ[ 4294965376 + gp ]) with
-            (mem' Ⓓ[ gp ⊖ 1920 ]); cycle 1. {
-            rewrite <- getmem_mod_l with (a := _ + _), <- setmem_mod_l.
-            rewrite getmem_noverlap. now unfold msub; psimpl.
-            replace (4294965376 ⊕ gp) with (gp ⊖ 1920) by
-                (now unfold msub; psimpl).
-            unfold addr_pxReadyTasksLists, uxTopReadyPriority.
-            replace (4 + _ ⊕ _) with ((gp ⊖ 920) ⊕ (31 ⊖ clz (mem' Ⓓ[ gp ⊖ 1920 ]) 32) * 20)
-                by (now unfold msub; psimpl).
-            auto.
-        } psimpl; unfold msub; simpl (_ - _); rewrite getmem_mod_l, (N.add_comm gp); psimpl; lia.
+    destruct PRE as [mem [MEM [GP [SP [A1 [A2 [A3 [A4 [A5 [NOVERLAPS
+        [PreservesPriority [Preserves920 [PreservesMem4 [NotSuspended 
+        [B1 Cycles]]]]]]]]]]]]]]].
+    destruct_noverlaps.
+    step. step. step. step. step. step. step. step. step. step. step.
+    unfold timing_postcondition.
+    (* unfold uxTopReadyPriority. noverlap_prepare gp sp. *)
+    replace (4 + (gp ⊖ 924) ⊕ (31 ⊖ clz (uxTopReadyPriority gp mem) 32) * 20) with
+        ((gp ⊖ 920) ⊕ (31 ⊖ clz (uxTopReadyPriority gp mem) 32) * 20) in BC by
+        (unfold msub; now psimpl).
+    rewrite <- Preserves920, <- PreservesPriority. 
+    apply Bool.negb_true_iff in BC.
+    rewrite BC, NotSuspended.
+    hammer. rewrite A1, A5.
+    replace (4 + _ ⊕ _) with ((gp ⊖ 920) ⊕ (31 ⊖ clz (mem Ⓓ[ gp ⊖ 1920 ]) 32) * 20)
+        by (unfold msub; now psimpl).
+    unfold uxTopReadyPriority in *. rewrite BC, Cycles.
+    cbn [negb]. psimpl. unfold msub in PreservesPriority.
+    psimpl in PreservesPriority. rewrite PreservesPriority. lia.
 
-    destruct PRE as [mem' [mem [gp [MEM [GP [SP [A2 [A3 [A4 [NOVERLAPS [NotSuspended
-        [BCPropagate Cycles]]]]]]]]]]]]. destruct_noverlaps.
-    step. step. step. step. step. step. step. step. step. step.
-        handle_ex. unfold timing_postcondition.
-        replace (uxSchedulerSuspended gp _ =? 0) with true.
-        hammer.
-        destruct (negb (mem' Ⓓ[ 4 + (gp ⊖ 924) ⊕ (31 ⊖ clz (uxTopReadyPriority gp mem') 32) * 20 ] 
-            =? gp ⊖ 916 ⊕ (31 ⊖ clz (uxTopReadyPriority gp mem') 32) * 20)) eqn:E.
-        { subst.
-            replace (_ =? _) with 
-            (mem' Ⓓ[ 4 + (gp ⊖ 924) ⊕ (31 ⊖ clz (uxTopReadyPriority gp mem') 32) * 20 ] =?
-                gp ⊖ 916 ⊕ (31 ⊖ clz (uxTopReadyPriority gp mem') 32) * 20).
-            apply Bool.negb_true_iff in E. rewrite E.
-            replace (mem' [Ⓓ _ := _] Ⓓ[ _ ]) with (mem' Ⓓ[ 4294965376 + gp ]).
-            rewrite Cycles. psimpl. lia.
-            now psimpl.
-            unfold uxTopReadyPriority, addr_pxReadyTasksLists.
-            rewrite <- setmem_mod_l.
-            replace (4294965400 ⊕ gp) with (gp ⊖ 1896); cycle 1. {
-                unfold msub. now psimpl.
-            }
-            rewrite <- getmem_mod_l with (a := _ + _ + _).
-            rewrite <- getmem_mod_l with (a := _ ⊖ _ + _).
-            (* rewrite <- setmem_mod_l with (a := _ + _ + _). *)
-            repeat rewrite getmem_noverlap.
-            unfold msub; now psimpl.
-            apply SMEM_WELL_FORMED; auto. discriminate.
-            apply noverlap_symmetry. auto.
-            apply SMEM_WELL_FORMED; auto. discriminate.
-        } destruct BCPropagate as [M920_912 [M912_M'912 M'920_M916]].
-        match goal with [|- context[if ?A then _ else _]] => 
-            replace A with true end.
-        rewrite <- getmem_mod_l, <- setmem_mod_l.
-        rewrite getmem_noverlap, Cycles. psimpl. rewrite getmem_mod_l. lia.
-            replace (4294965376 ⊕ gp) with (gp ⊖ 1920) by
-                (unfold msub; now psimpl).
-            replace (4294965400 ⊕ gp) with (gp ⊖ 1896) by
-                (unfold msub; now psimpl).
-            apply SMEM_WELL_FORMED; auto. discriminate.
-        {
-            unfold uxTopReadyPriority, addr_pxReadyTasksLists in *.
-            noverlap_prepare gp sp.
-            rewrite <- getmem_mod_l.
-            memsolve mem gp sp.
-            rewrite <- M'920_M916.
-            rewrite M912_M'912 in M920_912.
-            rewrite < 
-            rewrite M920_912.
-            apply noverlap_symmetry. auto.
-        }
-        noverlap_prepare gp n; memsolve mem gp n. now rewrite NotSuspended.
+    step. step. step. step. step. step. step. step. step. step. step. step.
+    unfold timing_postcondition.
+    apply Bool.negb_false_iff in BC.
+    replace (4 + _ ⊕ _) with ((gp ⊖ 920) ⊕ (31 ⊖ clz (mem Ⓓ[ gp ⊖ 1920 ]) 32) * 20)
+        in BC by (unfold msub; now psimpl).
+    unfold uxTopReadyPriority in *.
+    rewrite <- Preserves920, <- PreservesPriority, BC, NotSuspended.
+    hammer. rewrite A1, A5.
+    replace (4 + _ ⊕ _) with ((gp ⊖ 920) ⊕ (31 ⊖ clz (mem Ⓓ[ gp ⊖ 1920 ]) 32) * 20)
+        by (unfold msub; now psimpl).
+    unfold uxTopReadyPriority in *. rewrite BC, Cycles.
+    cbn [negb]. psimpl. unfold msub in PreservesPriority.
+    psimpl in PreservesPriority. rewrite PreservesPriority. lia.
+
     step. exact I.
 Admitted.
